hacspec/src/rustspec_to_fstar.rs
@@ -1,13 +1,17 @@
 use crate::rustspec::*;
 
+use crate::typechecker::{DictEntry, TypeDict};
 use core::iter::IntoIterator;
 use heck::SnakeCase;
 use pretty::RcDoc;
+use regex::Regex;
 use rustc_ast::ast::BinOpKind;
 use rustc_session::Session;
 use std::fs::File;
 use std::io::Write;
 use std::path;
+
+const SEQ_MODULE: &'static str = "RSeq";
 
 fn make_let_binding<'a>(
     pat: RcDoc<'a, ()>,
@@ -104,41 +108,46 @@ fn make_begin_paren<'a>(e: RcDoc<'a, ()>) -> RcDoc<'a, ()> {
 }
 
 fn translate_ident(x: &Ident) -> RcDoc<()> {
-    RcDoc::as_string(format!(
-        "{}",
-        match x {
-            Ident::Original(s) | Ident::Rustspec(_, s) => s.to_snake_case(),
-        }
-    ))
+    let mut ident_str = match x {
+        Ident::Original(s) => s.clone(),
+        Ident::Rustspec(id, s) => format!("{}_{}", s, id.0),
+    };
+    let secret_int_regex = Regex::new(r"(U|I)\d{1,3}").unwrap();
+    ident_str = secret_int_regex.replace_all(&ident_str, "s$0").to_string();
+    let mut snake_case_ident = ident_str.to_snake_case();
+    if snake_case_ident == "new" {
+        snake_case_ident = "new_".to_string();
+    }
+    RcDoc::as_string(snake_case_ident)
 }
 
 fn translate_base_typ(tau: &BaseTyp) -> RcDoc<()> {
     match tau {
         BaseTyp::Unit => RcDoc::as_string("unit"),
         BaseTyp::Bool => RcDoc::as_string("bool"),
-        BaseTyp::UInt8 => RcDoc::as_string("UInt8.t"),
-        BaseTyp::Int8 => RcDoc::as_string("Int8.t"),
-        BaseTyp::UInt16 => RcDoc::as_string("UInt16.t"),
-        BaseTyp::Int16 => RcDoc::as_string("Int16.t"),
-        BaseTyp::UInt32 => RcDoc::as_string("UInt32.t"),
-        BaseTyp::Int32 => RcDoc::as_string("Int32.t"),
-        BaseTyp::UInt64 => RcDoc::as_string("UInt64.t"),
-        BaseTyp::Int64 => RcDoc::as_string("Int64.t"),
-        BaseTyp::UInt128 => RcDoc::as_string("UInt128.t"),
-        BaseTyp::Int128 => RcDoc::as_string("Int128.t"),
-        BaseTyp::Usize => RcDoc::as_string("UInt32.t"),
-        BaseTyp::Isize => RcDoc::as_string("Int32.t"),
+        BaseTyp::UInt8 => RcDoc::as_string("u8"),
+        BaseTyp::Int8 => RcDoc::as_string("i8"),
+        BaseTyp::UInt16 => RcDoc::as_string("u16"),
+        BaseTyp::Int16 => RcDoc::as_string("i16"),
+        BaseTyp::UInt32 => RcDoc::as_string("u32"),
+        BaseTyp::Int32 => RcDoc::as_string("i32"),
+        BaseTyp::UInt64 => RcDoc::as_string("u64"),
+        BaseTyp::Int64 => RcDoc::as_string("i64"),
+        BaseTyp::UInt128 => RcDoc::as_string("u128"),
+        BaseTyp::Int128 => RcDoc::as_string("i128"),
+        BaseTyp::Usize => RcDoc::as_string("usize"),
+        BaseTyp::Isize => RcDoc::as_string("isize"),
         BaseTyp::Str => RcDoc::as_string("string"),
         BaseTyp::Seq(tau) => {
             let tau: &BaseTyp = &tau.0;
-            RcDoc::as_string("Seq.seq")
+            RcDoc::as_string(format!("{}.seq", SEQ_MODULE))
                 .append(RcDoc::space())
                 .append(translate_base_typ(tau))
                 .group()
         }
         BaseTyp::Array(size, tau) => {
             let tau: &BaseTyp = &tau.0;
-            RcDoc::as_string("Seq.lseq")
+            RcDoc::as_string(format!("{}.lseq", SEQ_MODULE))
                 .append(RcDoc::space())
                 .append(translate_base_typ(tau))
                 .append(RcDoc::space())
@@ -224,40 +233,75 @@ fn translate_unop(op: &UnOpKind) -> RcDoc<()> {
     }
 }
 
-fn translate_func_name<'a>(prefix: &'a Option<Spanned<BaseTyp>>, name: &'a Ident) -> RcDoc<'a, ()> {
+fn translate_prefix_for_func_name<'a, 'b>(
+    prefix: &'a BaseTyp,
+    typ_dict: &'a TypeDict,
+) -> (RcDoc<'a, ()>, Option<ArraySize>) {
+    match prefix {
+        BaseTyp::Bool => panic!(), // should not happen
+        BaseTyp::Unit => panic!(), // should not happen
+        BaseTyp::UInt8 => (RcDoc::as_string("RInt8"), None),
+        BaseTyp::Int8 => (RcDoc::as_string("RInt8"), None),
+        BaseTyp::UInt16 => (RcDoc::as_string("RUInt16"), None),
+        BaseTyp::Int16 => (RcDoc::as_string("RInt16"), None),
+        BaseTyp::UInt32 => (RcDoc::as_string("RUInt32"), None),
+        BaseTyp::Int32 => (RcDoc::as_string("RInt32"), None),
+        BaseTyp::UInt64 => (RcDoc::as_string("RUInt64"), None),
+        BaseTyp::Int64 => (RcDoc::as_string("RInt64"), None),
+        BaseTyp::UInt128 => (RcDoc::as_string("RUInt128"), None),
+        BaseTyp::Int128 => (RcDoc::as_string("RInt128"), None),
+        BaseTyp::Usize => (RcDoc::as_string("RUInt32"), None),
+        BaseTyp::Isize => (RcDoc::as_string("RInt32"), None),
+        BaseTyp::Str => (RcDoc::as_string("RString"), None),
+        BaseTyp::Seq(_) => (RcDoc::as_string(SEQ_MODULE), None),
+        BaseTyp::Array(size, _) => (RcDoc::as_string(SEQ_MODULE), Some(size.0.clone())),
+        BaseTyp::Named(ident, _) => {
+            // if the type is an array, we should print the Seq module instead
+            match &ident.0 {
+                Ident::Original(name) => match typ_dict.get(name) {
+                    Some((alias_typ, DictEntry::Array)) | Some((alias_typ, DictEntry::Alias)) => {
+                        translate_prefix_for_func_name(&(alias_typ.1).0, typ_dict)
+                    }
+                    _ => (RcDoc::as_string(name), None),
+                },
+                Ident::Rustspec(_, _) => panic!(), // should not happen
+            }
+        } // TODO: change with typ dict
+        BaseTyp::Variable(_) => panic!(), // shoult not happen
+        BaseTyp::Tuple(_) => panic!(),    // should not happen
+        BaseTyp::NaturalInteger(_, _) => unimplemented!(),
+    }
+}
+
+fn translate_func_name<'a>(
+    prefix: &'a Option<Spanned<BaseTyp>>,
+    name: &'a Ident,
+    typ_dict: &'a TypeDict,
+) -> RcDoc<'a, ()> {
     match prefix {
         None => translate_ident(name),
         Some((prefix, _)) => {
-            let module_name = match prefix {
-                BaseTyp::Bool => panic!(), // should not happen
-                BaseTyp::Unit => panic!(), // should not happen
-                BaseTyp::UInt8 => RcDoc::as_string("UInt8"),
-                BaseTyp::Int8 => RcDoc::as_string("Int8"),
-                BaseTyp::UInt16 => RcDoc::as_string("UInt16"),
-                BaseTyp::Int16 => RcDoc::as_string("Int16"),
-                BaseTyp::UInt32 => RcDoc::as_string("UInt32"),
-                BaseTyp::Int32 => RcDoc::as_string("Int32"),
-                BaseTyp::UInt64 => RcDoc::as_string("UInt64"),
-                BaseTyp::Int64 => RcDoc::as_string("Int64"),
-                BaseTyp::UInt128 => RcDoc::as_string("UInt128"),
-                BaseTyp::Int128 => RcDoc::as_string("Int128"),
-                BaseTyp::Usize => RcDoc::as_string("UInt32"),
-                BaseTyp::Isize => RcDoc::as_string("Int32"),
-                BaseTyp::Str => RcDoc::as_string("String"),
-                BaseTyp::Seq(_) | BaseTyp::Array(_, _) => RcDoc::as_string("Seq"),
-                BaseTyp::Named(_ident, _) => RcDoc::as_string("Seq"), // TODO: change with typ dict
-                BaseTyp::Variable(_) => panic!(),                     // shoult not happen
-                BaseTyp::Tuple(_) => panic!(),                        // should not happen
-                BaseTyp::NaturalInteger(_, _) => unimplemented!(),
-            };
+            let (module_name, array_size) = translate_prefix_for_func_name(prefix, typ_dict);
             let type_arg = match prefix {
                 BaseTyp::Seq(tau) => Some(translate_base_typ(&tau.0)),
                 BaseTyp::Array(_, tau) => Some(translate_base_typ(&tau.0)),
                 _ => None,
             };
+            let func_ident = translate_ident(name);
             module_name
                 .append(RcDoc::as_string("."))
-                .append(translate_ident(name))
+                .append(func_ident.clone())
+                .append(if format!("{}", func_ident.pretty(0)) == "new_" {
+                    match array_size {
+                        None => RcDoc::nil(),
+                        Some(ArraySize::Ident(s)) => RcDoc::space().append(RcDoc::as_string(s)),
+                        Some(ArraySize::Integer(i)) => {
+                            RcDoc::space().append(RcDoc::as_string(format!("{}ul", i)))
+                        }
+                    }
+                } else {
+                    RcDoc::nil()
+                })
                 .append(match type_arg {
                     None => RcDoc::nil(),
                     Some(arg) => RcDoc::space().append(RcDoc::as_string("#")).append(arg),
@@ -266,40 +310,45 @@ fn translate_func_name<'a>(prefix: &'a Option<Spanned<BaseTyp>>, name: &'a Ident
     }
 }
 
-fn translate_expression(e: &Expression) -> RcDoc<()> {
+fn translate_expression<'a>(e: &'a Expression, typ_dict: &'a TypeDict) -> RcDoc<'a, ()> {
     match e {
         Expression::Binary((op, _), ref e1, ref e2) => {
             let e1 = &e1.0;
             let e2 = &e2.0;
-            translate_expression(e1)
+            translate_expression(e1, typ_dict)
                 .append(RcDoc::space())
                 .append(translate_binop(op))
                 .append(RcDoc::space())
-                .append(translate_expression(e2))
+                .append(translate_expression(e2, typ_dict))
                 .group()
         }
         Expression::Unary(op, e1) => {
             let e1 = &e1.0;
             translate_unop(op)
                 .append(RcDoc::space())
-                .append(translate_expression(e1))
+                .append(translate_expression(e1, typ_dict))
                 .group()
         }
         Expression::Lit(lit) => translate_literal(lit),
-        Expression::Tuple(es) => make_tuple(es.into_iter().map(|(e, _)| translate_expression(&e))),
+        Expression::Tuple(es) => make_tuple(
+            es.into_iter()
+                .map(|(e, _)| translate_expression(&e, typ_dict)),
+        ),
         Expression::Named(p) => translate_ident(p),
-        Expression::FuncCall(prefix, name, args) => {
-            translate_func_name(prefix, &name.0).append(if args.len() > 0 {
+        Expression::FuncCall(prefix, name, args) => translate_func_name(prefix, &name.0, typ_dict)
+            .append(if args.len() > 0 {
                 RcDoc::concat(args.iter().map(|((arg, _), _)| {
-                    RcDoc::space().append(make_paren(translate_expression(arg)))
+                    RcDoc::space().append(make_paren(translate_expression(arg, typ_dict)))
                 }))
             } else {
                 RcDoc::space().append(RcDoc::as_string("()"))
-            })
-        }
-        Expression::MethodCall(_, _, (f, _), args) => translate_ident(f)
+            }),
+        Expression::MethodCall(sel_arg, _, (f, _), args) => translate_ident(f)
+            .append(
+                RcDoc::space().append(make_paren(translate_expression(&(sel_arg.0).0, typ_dict))),
+            )
             .append(RcDoc::concat(args.iter().map(|((arg, _), _)| {
-                RcDoc::space().append(make_paren(translate_expression(arg)))
+                RcDoc::space().append(make_paren(translate_expression(arg, typ_dict)))
             }))),
         Expression::ArrayIndex(x, e2) => {
             let e2 = &e2.0;
@@ -307,26 +356,31 @@ fn translate_expression(e: &Expression) -> RcDoc<()> {
                 .append(RcDoc::space())
                 .append(make_paren(translate_ident(&x.0)))
                 .append(RcDoc::space())
-                .append(make_paren(translate_expression(e2)))
+                .append(make_paren(translate_expression(e2, typ_dict)))
         }
-        Expression::NewArray(_, _, args) => RcDoc::as_string("Seq.from_list")
+        Expression::NewArray(_, _, args) => RcDoc::as_string(format!("{}.from_list", SEQ_MODULE))
             .append(RcDoc::space())
-            .append(make_list(args.iter().map(|(e, _)| translate_expression(e)))),
-        Expression::IntegerCasting(_, _) => panic!(),
+            .append(make_list(
+                args.iter().map(|(e, _)| translate_expression(e, typ_dict)),
+            )),
+        Expression::IntegerCasting(_, _) => unimplemented!(),
     }
 }
 
-fn translate_statement(s: &Statement) -> RcDoc<()> {
+fn translate_statement<'a>(s: &'a Statement, typ_dict: &'a TypeDict) -> RcDoc<'a, ()> {
     match s {
         Statement::LetBinding((pat, _), typ, (expr, _)) => make_let_binding(
             translate_pattern(pat),
             typ.as_ref().map(|(typ, _)| translate_typ(typ)),
-            translate_expression(expr),
+            translate_expression(expr, typ_dict),
             false,
         ),
-        Statement::Reassignment((x, _), (e1, _)) => {
-            make_let_binding(translate_ident(x), None, translate_expression(e1), false)
-        }
+        Statement::Reassignment((x, _), (e1, _)) => make_let_binding(
+            translate_ident(x),
+            None,
+            translate_expression(e1, typ_dict),
+            false,
+        ),
         Statement::ArrayUpdate((x, _), (e1, _), (e2, _)) => make_let_binding(
             translate_ident(x),
             None,
@@ -334,12 +388,12 @@ fn translate_statement(s: &Statement) -> RcDoc<()> {
                 .append(RcDoc::space())
                 .append(translate_ident(x))
                 .append(RcDoc::space())
-                .append(make_paren(translate_expression(e1)))
+                .append(make_paren(translate_expression(e1, typ_dict)))
                 .append(RcDoc::space())
-                .append(make_paren(translate_expression(e2))),
+                .append(make_paren(translate_expression(e2, typ_dict))),
             false,
         ),
-        Statement::ReturnExp(e1) => translate_expression(e1),
+        Statement::ReturnExp(e1) => translate_expression(e1, typ_dict),
         Statement::Conditional((cond, _), (b1, _), b2, mutated) => {
             let mutated_info = mutated.as_ref().unwrap().as_ref();
             make_let_binding(
@@ -347,27 +401,30 @@ fn translate_statement(s: &Statement) -> RcDoc<()> {
                 None,
                 RcDoc::as_string("if")
                     .append(RcDoc::space())
-                    .append(translate_expression(cond))
+                    .append(translate_expression(cond, typ_dict))
                     .append(RcDoc::space())
                     .append(RcDoc::as_string("then"))
                     .append(RcDoc::space())
                     .append(make_begin_paren(
-                        translate_block(b1, true)
+                        translate_block(b1, true, typ_dict)
                             .append(RcDoc::hardline())
-                            .append(translate_statement(&mutated_info.stmt)),
+                            .append(translate_statement(&mutated_info.stmt, typ_dict)),
                     ))
                     .append(match b2 {
                         None => RcDoc::space()
                             .append(RcDoc::as_string("else"))
                             .append(RcDoc::space())
-                            .append(make_begin_paren(translate_statement(&mutated_info.stmt))),
+                            .append(make_begin_paren(translate_statement(
+                                &mutated_info.stmt,
+                                typ_dict,
+                            ))),
                         Some((b2, _)) => RcDoc::space()
                             .append(RcDoc::as_string("else"))
                             .append(RcDoc::space())
                             .append(make_begin_paren(
-                                translate_block(b2, true)
+                                translate_block(b2, true, typ_dict)
                                     .append(RcDoc::hardline())
-                                    .append(translate_statement(&mutated_info.stmt)),
+                                    .append(translate_statement(&mutated_info.stmt, typ_dict)),
                             )),
                     }),
                 false,
@@ -379,9 +436,9 @@ fn translate_statement(s: &Statement) -> RcDoc<()> {
             let closure_tuple = make_tuple(vec![translate_ident(x), mut_tuple.clone()]);
             let loop_expr = RcDoc::as_string("foldi")
                 .append(RcDoc::space())
-                .append(make_paren(translate_expression(e1)))
+                .append(make_paren(translate_expression(e1, typ_dict)))
                 .append(RcDoc::space())
-                .append(make_paren(translate_expression(e2)))
+                .append(make_paren(translate_expression(e2, typ_dict)))
                 .append(RcDoc::space())
                 .append(RcDoc::as_string("(fun"))
                 .append(RcDoc::space())
@@ -389,9 +446,9 @@ fn translate_statement(s: &Statement) -> RcDoc<()> {
                 .append(RcDoc::space())
                 .append(RcDoc::as_string("->"))
                 .append(RcDoc::line())
-                .append(translate_block(b, true))
+                .append(translate_block(b, true, typ_dict))
                 .append(RcDoc::hardline())
-                .append(translate_statement(&mutated_info.stmt))
+                .append(translate_statement(&mutated_info.stmt, typ_dict))
                 .append(RcDoc::as_string(")"))
                 .group()
                 .nest(2)
@@ -403,9 +460,15 @@ fn translate_statement(s: &Statement) -> RcDoc<()> {
     .group()
 }
 
-fn translate_block(b: &Block, omit_extra_unit: bool) -> RcDoc<()> {
+fn translate_block<'a>(
+    b: &'a Block,
+    omit_extra_unit: bool,
+    typ_dict: &'a TypeDict,
+) -> RcDoc<'a, ()> {
     RcDoc::intersperse(
-        b.stmts.iter().map(|(i, _)| translate_statement(i).group()),
+        b.stmts
+            .iter()
+            .map(|(i, _)| translate_statement(i, typ_dict).group()),
         RcDoc::hardline(),
     )
     .append(match (&b.return_typ, omit_extra_unit) {
@@ -417,7 +480,7 @@ fn translate_block(b: &Block, omit_extra_unit: bool) -> RcDoc<()> {
     })
 }
 
-fn translate_item(i: &Item) -> RcDoc<()> {
+fn translate_item<'a>(i: &'a Item, typ_dict: &'a TypeDict) -> RcDoc<'a, ()> {
     match i {
         Item::FnDecl((f, _), sig, (b, _)) => make_let_binding(
             translate_ident(f)
@@ -446,7 +509,7 @@ fn translate_item(i: &Item) -> RcDoc<()> {
                         .group(),
                 ),
             None,
-            translate_block(b, false)
+            translate_block(b, false, typ_dict)
                 .append(if let BaseTyp::Unit = sig.ret.0 {
                     RcDoc::hardline().append(RcDoc::as_string("()"))
                 } else {
@@ -463,18 +526,18 @@ fn translate_item(i: &Item) -> RcDoc<()> {
             .group()
             .append(
                 RcDoc::line()
-                    .append(RcDoc::as_string("Seq.lseq"))
+                    .append(RcDoc::as_string(format!("{}.lseq", SEQ_MODULE)))
                     .append(RcDoc::space())
                     .append(translate_base_typ(&cell_t.0))
                     .append(RcDoc::space())
-                    .append(translate_expression(&size.0))
+                    .append(translate_expression(&size.0, typ_dict))
                     .group()
                     .nest(2),
             ),
         Item::ConstDecl(name, ty, e) => make_let_binding(
             translate_ident(&name.0),
             Some(translate_base_typ(&ty.0)),
-            translate_expression(&e.0),
+            translate_expression(&e.0, typ_dict),
             true,
         ),
         Item::NaturalIntegerDecl(_nat_name, canvas_name, _secrecy, canvas_size, _modulo) => {
@@ -490,25 +553,26 @@ fn translate_item(i: &Item) -> RcDoc<()> {
                         .append(RcDoc::space())
                         .append(translate_base_typ(&BaseTyp::UInt8))
                         .append(RcDoc::space())
-                        .append(translate_expression(&canvas_size.0))
+                        .append(translate_expression(&canvas_size.0, typ_dict))
                         .group()
                         .nest(2),
                 )
                 .append(RcDoc::hardline())
                 .append(RcDoc::hardline()) //TODO: add other decl
+                .append(RcDoc::as_string("// missing natural mod int type decl!"))
         }
     }
 }
 
-fn translate_program(p: &Program) -> RcDoc<()> {
+fn translate_program<'a>(p: &'a Program, typ_dict: &'a TypeDict) -> RcDoc<'a, ()> {
     RcDoc::concat(p.items.iter().map(|(i, _)| {
-        translate_item(i)
+        translate_item(i, typ_dict)
             .append(RcDoc::hardline())
             .append(RcDoc::hardline())
     }))
 }
 
-pub fn translate_and_write_to_file(sess: &Session, p: &Program, file: &str) {
+pub fn translate_and_write_to_file(sess: &Session, p: &Program, file: &str, typ_dict: &TypeDict) {
     let file = file.trim();
     let path = path::Path::new(file);
     let mut file = match File::create(&path) {
@@ -521,7 +585,14 @@ pub fn translate_and_write_to_file(sess: &Session, p: &Program, file: &str) {
     let width = 80;
     let mut w = Vec::new();
     let module_name = path.file_stem().unwrap().to_str().unwrap();
-    write!(file, "module {}\n\nopen Rustspec\n\n", module_name).unwrap();
-    translate_program(p).render(width, &mut w).unwrap();
+    write!(
+        file,
+        "module {}\n\nopen Rustspec\nopen FStar.Mul\n\nmodule RSeq = Rustspec.Seq\n\n",
+        module_name
+    )
+    .unwrap();
+    translate_program(p, typ_dict)
+        .render(width, &mut w)
+        .unwrap();
     write!(file, "{}", String::from_utf8(w).unwrap()).unwrap()
 }
