hacspec-fstar/Poly1305.fst
@@ -1,67 +1,82 @@
 module Poly1305
 
-module R = Rustspec
+open Rustspec
+open FStar.Mul
 
-let blocksize : UInt32.t =
+module RSeq = Rustspec.Seq
+
+let blocksize : usize =
   16ul
 
-type block = Seq.lseq u8 blocksize
+type block = RSeq.lseq s_u8 blocksize
 
-type tag = Seq.lseq UInt8.t blocksize
+type tag = RSeq.lseq u8 blocksize
 
-type field_canvas = Seq.lseq UInt8.t 272ul
+type field_canvas = Seq.lseq u8 272ul
 
+// missing natural mod int type decl!
 
+let key_gen (key_1885 : key) (iv_1886 : iv) : key =
+  let block_1887 = block (key_1885) (s_u32 (0ul)) (iv_1886) in
+  RSeq.from_slice_range (block_1887) ((0ul, 32ul))
 
-let key_gen (key : key) (iv : iv) : key =
-  let block = block (key) (u32 (0ul)) (iv) in
-  Seq.from_slice_range (block) ((0ul, 32ul))
-
-let encode_r (r : block) : field_element =
-  let r_128 = Seq.from_slice (r) (0ul) (blocksize) in
-  let r_uint = u128_from_le_bytes (r_128) in
-  let r_uint =
-    r_uint & u128 (UInt128.uint_to_t 21267647620597763993911028882763415551)
+let encode_r (r_1888 : block) : field_element =
+  let r_128_1889 = RSeq.from_slice (r_1888) (0ul) (blocksize) in
+  let r_uint_1890 = s_u128_from_le_bytes (r_128_1889) in
+  let r_uint_1891 =
+    r_uint_1890 & s_u128 (
+      UInt128.uint_to_t 21267647620597763993911028882763415551)
   in
-  Seq.from_secret_literal (r_uint)
+  FieldElement.from_secret_literal (r_uint_1891)
 
-let encode (block : byte_seq) : field_element =
-  let block_len = len in
-  let block_as_u128 = Seq.from_slice (block) (0ul) (min (16ul) (block_len)) in
-  let w_elem = Seq.from_secret_literal (u128_from_le_bytes (block_as_u128)) in
-  let l_elem = Seq.from_canvas (Seq.pow2 (8ul * block_len)) in
-  w_elem + l_elem
-
-let poly_inner (m : byte_seq) (r : field_element) : field_element =
-  let acc = Seq.from_literal (UInt128.uint_to_t 0) in
-  let (acc) =
-    foldi (0ul) (num_chunks (blocksize)) (fun (i, (acc)) ->
-      let (_, block) = get_chunk (blocksize) (i) in
-      let acc = acc + encode (block) * r in
-      (acc))
-    (acc)
+let encode (block_1892 : byte_seq) : field_element =
+  let block_len_1893 = len (block_1892) in
+  let block_as_u128_1894 =
+    RSeq.from_slice (block_1892) (0ul) (min (16ul) (block_len_1893))
   in
-  acc
-
-let poly (m : byte_seq) (key : key) : tag =
-  let s_elem =
-    Seq.from_secret_literal (
-      u128_from_le_bytes (Seq.from_slice (key) (blocksize) (blocksize)))
+  let w_elem_1895 =
+    FieldElement.from_secret_literal (s_u128_from_le_bytes (block_as_u128_1894))
   in
-  let r_elem = encode_r (Seq.from_slice_range (key) ((0ul, blocksize))) in
-  let a = poly_inner (m) (r_elem) in
-  let n = a + s_elem in
-  let n_v = to_public_byte_seq_le in
-  let tag = Seq.new () in
-  let (tag) =
-    foldi (0ul) (min (len) (len)) (fun (i, (tag)) ->
-      let tag = array_upd tag (i) (array_index (n_v) (i)) in
-      (tag))
-    (tag)
+  let l_elem_1896 =
+    FieldElement.from_canvas (RSeq.pow2 (8ul * block_len_1893))
   in
-  tag
+  w_elem_1895 + l_elem_1896
 
-let poly_mac (m : byte_seq) (key : key) (iv : iv) : tag =
-  let mac_key = key_gen (key) (iv) in
-  poly (m) (mac_key)
+let poly_inner (m_1897 : byte_seq) (r_1898 : field_element) : field_element =
+  let acc_1899 = FieldElement.from_literal (UInt128.uint_to_t 0) in
+  let (acc_1899) =
+    foldi (0ul) (num_chunks (m_1897) (blocksize)) (fun (i_1900, (acc_1899)) ->
+      let (_, block_1901) = get_chunk (m_1897) (blocksize) (i_1900) in
+      let acc_1899 = acc_1899 + encode (block_1901) * r_1898 in
+      (acc_1899))
+    (acc_1899)
+  in
+  acc_1899
+
+let poly (m_1902 : byte_seq) (key_1903 : key) : tag =
+  let s_elem_1904 =
+    FieldElement.from_secret_literal (
+      s_u128_from_le_bytes (RSeq.from_slice (key_1903) (blocksize) (blocksize)))
+  in
+  let r_elem_1905 =
+    encode_r (RSeq.from_slice_range (key_1903) ((0ul, blocksize)))
+  in
+  let a_1906 = poly_inner (m_1902) (r_elem_1905) in
+  let n_1907 = a_1906 + s_elem_1904 in
+  let n_v_1908 = to_public_byte_seq_le (n_1907) in
+  let tag_1909 = RSeq.new_ BLOCKSIZE () in
+  let (tag_1909) =
+    foldi (0ul) (min (len (tag_1909)) (len (n_v_1908))) (fun (i_1910, (tag_1909)
+      ) ->
+      let tag_1909 =
+        array_upd tag_1909 (i_1910) (array_index (n_v_1908) (i_1910))
+      in
+      (tag_1909))
+    (tag_1909)
+  in
+  tag_1909
+
+let poly_mac (m_1911 : byte_seq) (key_1912 : key) (iv_1913 : iv) : tag =
+  let mac_key_1914 = key_gen (key_1912) (iv_1913) in
+  poly (m_1911) (mac_key_1914)
 
