hacspec-fstar/Chacha20.fst
@@ -1,124 +1,152 @@
 module Chacha20
 
 open Rustspec
+open FStar.Mul
 
-type state = Seq.lseq u32 16ul
+module RSeq = Rustspec.Seq
 
-type state_bytes = Seq.lseq u8 64ul
+type state = RSeq.lseq s_u32 16ul
 
-type iv = Seq.lseq u8 12ul
+type state_bytes = RSeq.lseq s_u8 64ul
 
-type key = Seq.lseq u8 32ul
+type iv = RSeq.lseq s_u8 12ul
 
-let state_to_bytes (x : state) : state_bytes =
-  let r = Seq.new () in
-  let (r) =
-    foldi (0ul) (len) (fun (i, (r)) ->
-      let bytes = u32_to_be_bytes (array_index (x) (i)) in
-      let r = array_upd r (i * 4ul) (array_index (bytes) (3ul)) in
-      let r = array_upd r (i * 4ul + 1ul) (array_index (bytes) (2ul)) in
-      let r = array_upd r (i * 4ul + 2ul) (array_index (bytes) (1ul)) in
-      let r = array_upd r (i * 4ul + 3ul) (array_index (bytes) (0ul)) in
-      (r))
-    (r)
+type key = RSeq.lseq s_u8 32ul
+
+let state_to_bytes (x_1870 : state) : state_bytes =
+  let r_1871 = RSeq.new_ 64ul () in
+  let (r_1871) =
+    foldi (0ul) (len (x_1870)) (fun (i_1872, (r_1871)) ->
+      let bytes_1873 = s_u32_to_be_bytes (array_index (x_1870) (i_1872)) in
+      let r_1871 =
+        array_upd r_1871 (i_1872 * 4ul) (array_index (bytes_1873) (3ul))
+      in
+      let r_1871 =
+        array_upd r_1871 (i_1872 * 4ul + 1ul) (array_index (bytes_1873) (2ul))
+      in
+      let r_1871 =
+        array_upd r_1871 (i_1872 * 4ul + 2ul) (array_index (bytes_1873) (1ul))
+      in
+      let r_1871 =
+        array_upd r_1871 (i_1872 * 4ul + 3ul) (array_index (bytes_1873) (0ul))
+      in
+      (r_1871))
+    (r_1871)
   in
-  r
+  r_1871
 
 let line
-  (a : UInt32.t)
-  (b : UInt32.t)
-  (d : UInt32.t)
-  (s : UInt32.t)
-  (m : state)
+  (a_1874 : u32)
+  (b_1875 : u32)
+  (d_1876 : u32)
+  (s_1877 : usize)
+  (m_1878 : state)
   : state =
-  let state = m in
-  let state =
-    array_upd state (a) (array_index (state) (a) + array_index (state) (b))
+  let state_1879 = m_1878 in
+  let state_1879 =
+    array_upd state_1879 (a_1874) (
+      array_index (state_1879) (a_1874) + array_index (state_1879) (b_1875))
   in
-  let state =
-    array_upd state (d) (array_index (state) (d) ^ array_index (state) (a))
+  let state_1879 =
+    array_upd state_1879 (d_1876) (
+      array_index (state_1879) (d_1876) ^ array_index (state_1879) (a_1874))
   in
-  let state = array_upd state (d) (rotate_left (s)) in
-  state
+  let state_1879 =
+    array_upd state_1879 (d_1876) (
+      rotate_left (array_index (state_1879) (d_1876)) (s_1877))
+  in
+  state_1879
 
 let quarter_round
-  (a : UInt32.t)
-  (b : UInt32.t)
-  (c : UInt32.t)
-  (d : UInt32.t)
-  (state : state)
+  (a_1880 : u32)
+  (b_1881 : u32)
+  (c_1882 : u32)
+  (d_1883 : u32)
+  (state_1884 : state)
   : state =
-  let state = line (a) (b) (d) (16ul) (state) in
-  let state = line (c) (d) (b) (12ul) (state) in
-  let state = line (a) (b) (d) (8ul) (state) in
-  line (c) (d) (b) (7ul) (state)
+  let state_1885 = line (a_1880) (b_1881) (d_1883) (16ul) (state_1884) in
+  let state_1886 = line (c_1882) (d_1883) (b_1881) (12ul) (state_1885) in
+  let state_1887 = line (a_1880) (b_1881) (d_1883) (8ul) (state_1886) in
+  line (c_1882) (d_1883) (b_1881) (7ul) (state_1887)
 
-let double_round (state : state) : state =
-  let state = quarter_round (0ul) (4ul) (8ul) (12ul) (state) in
-  let state = quarter_round (1ul) (5ul) (9ul) (13ul) (state) in
-  let state = quarter_round (2ul) (6ul) (10ul) (14ul) (state) in
-  let state = quarter_round (3ul) (7ul) (11ul) (15ul) (state) in
-  let state = quarter_round (0ul) (5ul) (10ul) (15ul) (state) in
-  let state = quarter_round (1ul) (6ul) (11ul) (12ul) (state) in
-  let state = quarter_round (2ul) (7ul) (8ul) (13ul) (state) in
-  quarter_round (3ul) (4ul) (9ul) (14ul) (state)
+let double_round (state_1888 : state) : state =
+  let state_1889 = quarter_round (0ul) (4ul) (8ul) (12ul) (state_1888) in
+  let state_1890 = quarter_round (1ul) (5ul) (9ul) (13ul) (state_1889) in
+  let state_1891 = quarter_round (2ul) (6ul) (10ul) (14ul) (state_1890) in
+  let state_1892 = quarter_round (3ul) (7ul) (11ul) (15ul) (state_1891) in
+  let state_1893 = quarter_round (0ul) (5ul) (10ul) (15ul) (state_1892) in
+  let state_1894 = quarter_round (1ul) (6ul) (11ul) (12ul) (state_1893) in
+  let state_1895 = quarter_round (2ul) (7ul) (8ul) (13ul) (state_1894) in
+  quarter_round (3ul) (4ul) (9ul) (14ul) (state_1895)
 
-let block_init (key : key) (ctr : u32) (iv : iv) : state =
-  Seq.from_list [
-    u32 (1634760805ul);
-    u32 (857760878ul);
-    u32 (2036477234ul);
-    u32 (1797285236ul);
-    u32_from_le_bytes (Seq.from_slice_range (key) ((0ul, 4ul)));
-    u32_from_le_bytes (Seq.from_slice_range (key) ((4ul, 8ul)));
-    u32_from_le_bytes (Seq.from_slice_range (key) ((8ul, 12ul)));
-    u32_from_le_bytes (Seq.from_slice_range (key) ((12ul, 16ul)));
-    u32_from_le_bytes (Seq.from_slice_range (key) ((16ul, 20ul)));
-    u32_from_le_bytes (Seq.from_slice_range (key) ((20ul, 24ul)));
-    u32_from_le_bytes (Seq.from_slice_range (key) ((24ul, 28ul)));
-    u32_from_le_bytes (Seq.from_slice_range (key) ((28ul, 32ul)));
-    ctr;
-    u32_from_le_bytes (Seq.from_slice_range (iv) ((0ul, 4ul)));
-    u32_from_le_bytes (Seq.from_slice_range (iv) ((4ul, 8ul)));
-    u32_from_le_bytes (Seq.from_slice_range (iv) ((8ul, 12ul)))
+let block_init (key_1896 : key) (ctr_1897 : s_u32) (iv_1898 : iv) : state =
+  RSeq.from_list [
+    s_u32 (1634760805ul);
+    s_u32 (857760878ul);
+    s_u32 (2036477234ul);
+    s_u32 (1797285236ul);
+    s_u32_from_le_bytes (RSeq.from_slice_range (key_1896) ((0ul, 4ul)));
+    s_u32_from_le_bytes (RSeq.from_slice_range (key_1896) ((4ul, 8ul)));
+    s_u32_from_le_bytes (RSeq.from_slice_range (key_1896) ((8ul, 12ul)));
+    s_u32_from_le_bytes (RSeq.from_slice_range (key_1896) ((12ul, 16ul)));
+    s_u32_from_le_bytes (RSeq.from_slice_range (key_1896) ((16ul, 20ul)));
+    s_u32_from_le_bytes (RSeq.from_slice_range (key_1896) ((20ul, 24ul)));
+    s_u32_from_le_bytes (RSeq.from_slice_range (key_1896) ((24ul, 28ul)));
+    s_u32_from_le_bytes (RSeq.from_slice_range (key_1896) ((28ul, 32ul)));
+    ctr_1897;
+    s_u32_from_le_bytes (RSeq.from_slice_range (iv_1898) ((0ul, 4ul)));
+    s_u32_from_le_bytes (RSeq.from_slice_range (iv_1898) ((4ul, 8ul)));
+    s_u32_from_le_bytes (RSeq.from_slice_range (iv_1898) ((8ul, 12ul)))
   ]
 
-let block_inner (key : key) (ctr : u32) (iv : iv) : state =
-  let st = block_init (key) (ctr) (iv) in
-  let state = st in
-  let (state) =
-    foldi (0ul) (10ul) (fun (i, (state)) ->
-      let state = double_round (state) in
-      (state))
-    (state)
+let block_inner (key_1899 : key) (ctr_1900 : s_u32) (iv_1901 : iv) : state =
+  let st_1902 = block_init (key_1899) (ctr_1900) (iv_1901) in
+  let state_1903 = st_1902 in
+  let (state_1903) =
+    foldi (0ul) (10ul) (fun (i_1904, (state_1903)) ->
+      let state_1903 = double_round (state_1903) in
+      (state_1903))
+    (state_1903)
   in
-  let (state) =
-    foldi (0ul) (16ul) (fun (i, (state)) ->
-      let state =
-        array_upd state (i) (array_index (state) (i) + array_index (st) (i))
+  let (state_1903) =
+    foldi (0ul) (16ul) (fun (i_1905, (state_1903)) ->
+      let state_1903 =
+        array_upd state_1903 (i_1905) (
+          array_index (state_1903) (i_1905) + array_index (st_1902) (i_1905))
       in
-      (state))
-    (state)
+      (state_1903))
+    (state_1903)
   in
-  state
+  state_1903
 
-let block (key : key) (ctr : u32) (iv : iv) : state_bytes =
-  let state = block_inner (key) (ctr) (iv) in
-  state_to_bytes (state)
+let block (key_1906 : key) (ctr_1907 : s_u32) (iv_1908 : iv) : state_bytes =
+  let state_1909 = block_inner (key_1906) (ctr_1907) (iv_1908) in
+  state_to_bytes (state_1909)
 
-let chacha (key : key) (iv : iv) (m : byte_seq) : byte_seq =
-  let ctr = u32 (1ul) in
-  let blocks_out = Seq.new (len) in
-  let (blocks_out, ctr) =
-    foldi (0ul) (num_chunks (64ul)) (fun (i, (blocks_out, ctr)) ->
-      let (block_len, msg_block) = get_chunk (64ul) (i) in
-      let key_block = block (key) (ctr) (iv) in
-      let msg_block_padded = Seq.new () in
-      let msg_block_padded = update_start (msg_block) in
-      let blocks_out = set_chunk (64ul) (i) (slice_range ((0ul, block_len))) in
-      let ctr = ctr + u32 (1ul) in
-      (blocks_out, ctr))
-    (blocks_out, ctr)
+let chacha (key_1910 : key) (iv_1911 : iv) (m_1912 : byte_seq) : byte_seq =
+  let ctr_1913 = s_u32 (1ul) in
+  let blocks_out_1914 = RSeq.new_ (len (m_1912)) in
+  let (blocks_out_1914, ctr_1913) =
+    foldi (0ul) (num_chunks (m_1912) (64ul)) (fun (
+        i_1915,
+        (blocks_out_1914, ctr_1913)
+      ) ->
+      let (block_len_1916, msg_block_1917) =
+        get_chunk (m_1912) (64ul) (i_1915)
+      in
+      let key_block_1918 = block (key_1910) (ctr_1913) (iv_1911) in
+      let msg_block_padded_1919 = RSeq.new_ 64ul () in
+      let msg_block_padded_1920 =
+        update_start (msg_block_padded_1919) (msg_block_1917)
+      in
+      let blocks_out_1914 =
+        set_chunk (blocks_out_1914) (64ul) (i_1915) (
+          slice_range (msg_block_padded_1920 ^ key_block_1918) (
+            (0ul, block_len_1916)))
+      in
+      let ctr_1913 = ctr_1913 + s_u32 (1ul) in
+      (blocks_out_1914, ctr_1913))
+    (blocks_out_1914, ctr_1913)
   in
-  blocks_out
+  blocks_out_1914
 
