hacspec-fstar/Rustspec.Loop.fst
@@ -1,0 +1,5 @@
+module Rustspec.Loop
+
+open Rustspec.Int
+
+assume val foldi (#acc: Type) (lo: usize) (hi: usize) (f: (usize & acc) -> acc) (init: acc) : acc
