hacspec-fstar/Rustspec.Seq.fst
@@ -1,0 +1,14 @@
+module Rustspec.Seq
+
+open Rustspec.Int
+
+type lseq (a: Type) (len: usize) = FStar.Seq.lseq a (UInt32.v len)
+
+assume val new_ (#a: Type) (len: usize) (_: unit) : lseq a len
+
+assume val array_index (#a: Type) (#len: usize) (s: lseq a len) (i: usize{UInt32.v i < UInt32.v len}) : a
+
+assume val array_upd (#a: Type) (#len: usize) (s: lseq a len) (i: usize{UInt32.v i < UInt32.v len})
+ (new_v: a) : lseq a len
+
+let len (#a: Type) (#len: usize) (s: lseq a len) = len
