hacspec-fstar/Rustspec.fst
@@ -1,1 +1,5 @@
 module Rustspec
+
+include Rustspec.Int
+include Rustspec.Seq
+include Rustspec.Loop
